Affine/Conversion.lean
@@ -3,12 +3,14 @@ import «Affine».Misc
 
 namespace Affine
 
+/-- Converts an `e : Affine vs` to a `Lambda`. -/
 def to_lambda (e : Affine vs) : Lambda :=
   match e with
   | .var x => .var x
   | .abs x e => .abs x e.to_lambda
   | .app e₁ e₂ _ => .app e₁.to_lambda e₂.to_lambda
 
+/-- Converts an affine `e : Lambda` to an `Affine e.free`. -/
 def of_lambda {e : Lambda} (h : e.is_affine) : Affine e.free :=
   match e with
   | .var x => .var x
@@ -17,6 +19,7 @@ def of_lambda {e : Lambda} (h : e.is_affine) : Affine e.free :=
     have ⟨he₁, he₂, hinter⟩ := Lambda.is_affine_of_app.mp h
     .app (Affine.of_lambda he₁) (Affine.of_lambda he₂) hinter
 
+/-- Conversions preserve free variables. -/
 theorem to_lambda_free_eq (e : Affine vs) : e.free = e.to_lambda.free := by
   match e with
   | .var x => simp only [free, to_lambda, Lambda.free]
@@ -24,6 +27,7 @@ theorem to_lambda_free_eq (e : Affine vs) : e.free = e.to_lambda.free := by
   | .app e₁ e₂ h =>
     simp only [free, to_lambda, Lambda.free, to_lambda_free_eq e₁, to_lambda_free_eq e₂]
 
+/-- Conversions preserve counts. -/
 theorem to_lambda_count_eq (e : Affine vs) : e.count x = e.to_lambda.count x := by
   match e with
   | .var x' => simp only [count, to_lambda, Lambda.count]
@@ -31,6 +35,7 @@ theorem to_lambda_count_eq (e : Affine vs) : e.count x = e.to_lambda.count x := 
   | .app e₁ e₂ h =>
     simp only [count, to_lambda, Lambda.count, to_lambda_count_eq e₁, to_lambda_count_eq e₂]
 
+/-- Conversions preserve affinity. -/
 theorem to_lambda_is_affine (e : Affine vs) : e.to_lambda.is_affine := by
   match e with
   | .var x => simp only [to_lambda, Lambda.is_affine]
@@ -43,4 +48,17 @@ theorem to_lambda_is_affine (e : Affine vs) : e.to_lambda.is_affine := by
       to_lambda_is_affine e₁, to_lambda_is_affine e₂, true_and, decide_eq_true_eq,
       ← to_lambda_free_eq e₁, ← to_lambda_free_eq e₂, h]
 
+theorem to_lambda_count_β_eq (e : Affine vs) : e.to_lambda.count_β = e.count_β := by sorry
+
+theorem of_lambda_count_β_eq {e : Lambda} (h : e.is_affine) :
+    (Affine.of_lambda h).count_β = e.count_β := by sorry
+
 end Affine
+
+namespace Lambda
+
+theorem of_lambda_to_lambda {e : Lambda} (h : e.is_affine) :
+    (Affine.of_lambda h).to_lambda = e := by
+  sorry
+
+end Lambda
