readme.md
@@ -1,0 +1,46 @@
+# Affine Lambda Calculus in Lean
+
+## Definitions
+- [`Affine`][1] are affine lambda terms:
+```
+/--
+  Affine lambda terms, where bound variables can be used at most once.
+
+  The choice of `Finset` over:
+  - `List`: Can have duplicates.
+  - `Set`: Can be infinite.
+-/
+inductive Affine : (vs : Finset ℕ) → Type
+| var (x : ℕ) : Affine {x}
+| abs (x : ℕ) (e : Affine vs) : Affine (vs \ {x})
+| app (e₁ : Affine vs₁) (e₂ : Affine vs₂) (h : vs₁ ∩ vs₂ = ∅) : Affine (vs₁ ∪ vs₂)
+```
+This definition tracks the free variables and ensures affinity.
+
+- [`Lambda`][2] are general lambda terms, which don't track their free variables:
+```
+inductive Lambda : Type
+| var (x : ℕ) : Lambda
+| abs (x : ℕ) (e : Lambda) : Lambda
+| app (e₁ : Lambda) (e₂ : Lambda) : Lambda
+```
+
+## Normalization
+In [`Normalize.lean`][3] we define `Affine.normalize`, which repeatedly applies
+β-reductions until none are left. This is done by first converting the `Affine` term
+to a `Lambda` term, since typing is easier there.
+
+Terminations is proven by counting the nubmer of β-reductions remaining, which always
+decreases after an application of `small_step`, unless there are none.
+
+In [`Normalize.lean`][3], we also have `Affine.normalize_is_normal`, which proves that,
+after normalizing, no β-reductions remain.
+
+## TODO
+In retrospect I should have used [De Bruijn index][4] in order to side-step the complications
+when renaming variables during substitutions.
+
+[1]: ./Affine/Affine.lean
+[2]: ./Affine/Lambda.lean
+[3]: ./Affine/Normalize.lean
+[4]: https://en.wikipedia.org/wiki/De_Bruijn_index
